simplify state model formalization
Use records instead of tuples. Do not impose on the type itself that fields can be at most 1 permission --> need to handle this now via a separate predicate in the semantics (this is also more flexible if one wanted to put this as part of the state consistency parameter).

TotalStateUtil.thy
@@ -1,11 +1,11 @@
 theory TotalStateUtil
-imports TotalViperState
+imports TotalViperState Viper.DeBruijn
 begin
 
 section \<open>update_store_total\<close>
 
 fun update_var_total :: "'a full_total_state \<Rightarrow> var \<Rightarrow> 'a val \<Rightarrow> 'a full_total_state"
-  where "update_var_total \<omega> x v = ((get_store_total \<omega>)(x \<mapsto> v), get_trace_total \<omega>, get_total_full \<omega>)"
+  where "update_var_total \<omega> x v = \<omega>\<lparr>get_store_total := (get_store_total \<omega>)(x \<mapsto> v)\<rparr>"
 
 lemma update_var_total_trace_eq: "get_trace_total (update_var_total \<omega> x v) = get_trace_total \<omega>"
   by simp
@@ -20,12 +20,12 @@ lemma update_var_total_mask_same: "get_total_full (update_var_total \<omega> x v
   by simp
 
 fun update_store_total :: "'a full_total_state \<Rightarrow> 'a store \<Rightarrow> 'a full_total_state"
-  where "update_store_total \<omega> \<sigma> = (\<sigma>, get_trace_total \<omega>, get_total_full \<omega>)"
+  where "update_store_total \<omega> \<sigma> = \<omega>\<lparr>get_store_total := \<sigma>\<rparr>"
 
 section \<open>update_trace_total\<close>
 
 fun update_trace_total :: "'a full_total_state \<Rightarrow> 'a total_trace \<Rightarrow> 'a full_total_state"
-  where "update_trace_total \<omega> \<pi> = (get_store_total \<omega>, \<pi>, get_total_full \<omega>)"
+  where "update_trace_total \<omega> \<pi> = \<omega>\<lparr>get_trace_total := \<pi>\<rparr>"
 
 lemma update_trace_total_store_same: "get_store_total (update_trace_total \<omega> \<pi>) = get_store_total \<omega>"
   by simp
@@ -42,24 +42,28 @@ lemma update_trace_total_mask_same: "get_mh_total_full (update_trace_total \<ome
 section \<open>update heap and mask total\<close>
 
 definition update_hh_loc_total :: "'a total_state \<Rightarrow> heap_loc \<Rightarrow> 'a val \<Rightarrow> 'a total_state"
-  where "update_hh_loc_total \<phi> l v = Abs_total_state (((get_hh_total \<phi>)(l := v), get_hp_total \<phi>), get_m_total \<phi>)"
+  where "update_hh_loc_total \<phi> l v = \<phi>\<lparr>get_hh_total := (get_hh_total \<phi>)(l := v)\<rparr>"
 
 definition update_mh_total :: "'a total_state \<Rightarrow> mask \<Rightarrow> 'a total_state"
-  where "update_mh_total \<phi> mh = Abs_total_state (get_h_total \<phi>, (mh, get_mp_total \<phi>))"
+  where "update_mh_total \<phi> mh = \<phi>\<lparr>get_mh_total := mh\<rparr>"
 
 definition update_mp_total :: "'a total_state \<Rightarrow> 'a predicate_mask \<Rightarrow> 'a total_state"
-  where "update_mp_total \<phi> mp = Abs_total_state (get_h_total \<phi>, (get_mh_total \<phi>, mp))"
+  where "update_mp_total \<phi> mp = \<phi>\<lparr>get_mp_total := mp\<rparr>"
 
+(*
 definition update_m_total :: "'a total_state \<Rightarrow> mask \<times> 'a predicate_mask \<Rightarrow> 'a total_state"
   where "update_m_total \<phi> m = Abs_total_state (get_h_total \<phi>, m)"
+*)
 
-
+(*
 lemma Abs_total_state_inverse_2:
   assumes "wf_pre_total_state (m,h)"
   shows "Rep_total_state (Abs_total_state (m,h)) = (m,h)"
   using assms Abs_total_state_inverse
   by blast
+*)
 
+(*
 lemma get_m_update_m_total:
   assumes "wf_mask_simple (fst m)"
   shows "get_m_total (update_m_total \<phi> m) = m"
@@ -83,27 +87,28 @@ lemma update_m_total_eq:
    apply (simp only: get_m_update_m_total[OF assms(1)])
   apply (simp only: get_h_update_m_total[OF assms(1)] assms(2))
   done
-  
+*)
+
 lemma get_update_mh_total: 
   assumes "wf_mask_simple m0"
   shows   "get_mh_total (update_mh_total mh m0) = m0"
   unfolding update_mh_total_def
   using assms
-  by (simp add: Abs_total_state_inverse_2)
+  by simp
 
 lemma update_mh_total_multiple: 
-  assumes "wf_mask_simple m0" and "wf_mask_simple m2"
   shows   "update_mh_total (update_mh_total mh m0) m1 = update_mh_total mh m1"
   unfolding update_mh_total_def  
-  using assms
-  by (simp add: Abs_total_state_inverse_2)
+  by simp
 
+(*
 lemma wf_pre_total_state_1: 
   assumes"get_mh_pre_total \<phi>' = get_mh_total \<phi>"
   shows "wf_pre_total_state \<phi>'"
   using assms
   using get_mask_total_wf by fastforce
-
+*)
+(*
 lemma update_hh_loc_total_m_eq: "get_m_total (update_hh_loc_total \<phi> l v) = get_m_total \<phi>"
   unfolding update_hh_loc_total_def
 proof -
@@ -114,45 +119,28 @@ proof -
   thus "get_m_total (Abs_total_state ?\<phi>') = (get_m_total \<phi>)"
     by (simp add: Abs_total_state_inverse_2)
 qed
+*)
 
+(*
 lemma m_eq_mh_eq_total: "get_m_total \<phi> = get_m_total \<phi>' \<Longrightarrow> get_mh_total \<phi> = get_mh_total \<phi>'"
   by simp
 
 lemma m_eq_mp_eq_total: "get_m_total \<phi> = get_m_total \<phi>' \<Longrightarrow> get_mp_total \<phi> = get_mp_total \<phi>'"
   by simp
+*)
 
 lemma update_hh_loc_total_mh_eq: "get_mh_total (update_hh_loc_total \<phi> l v) = get_mh_total \<phi>"
-  using m_eq_mh_eq_total update_hh_loc_total_m_eq
-  by blast
+  by (simp add: update_hh_loc_total_def)
 
 lemma update_hh_loc_total_mp_eq: "get_mp_total (update_hh_loc_total \<phi> l v) = get_mp_total \<phi>"
-  using m_eq_mp_eq_total update_hh_loc_total_m_eq
-  by blast
+  by (simp add: update_hh_loc_total_def)
 
 lemma update_hh_loc_total_hp_eq: "get_hp_total (update_hh_loc_total \<phi> l v) = get_hp_total \<phi>"
   unfolding update_hh_loc_total_def
-proof -
-  let ?\<phi>' = "(((get_hh_total \<phi>)(l := v), get_hp_total \<phi>), get_m_total \<phi>)"
-  have "wf_pre_total_state ?\<phi>'"
-    apply (rule wf_pre_total_state_1[where ?\<phi>=\<phi>])
-    by simp
-  thus "get_hp_total (Abs_total_state ?\<phi>') = (get_hp_total \<phi>)"
-    by (simp add: Abs_total_state_inverse_2)
-qed
-
-lemma Rep_total_state_inj: "Rep_total_state a = Rep_total_state b \<Longrightarrow> a = b"
-  by (metis Rep_total_state_inverse)
+  by simp
 
 lemma update_hh_loc_total_fupd: "get_hh_total (update_hh_loc_total \<phi> l1 v) = (get_hh_total \<phi>)(l1 := v)"
-  unfolding update_hh_loc_total_def
-proof -
-  let ?\<phi>'="(((get_hh_total \<phi>)(l1 := v), get_hp_total \<phi>), get_m_total \<phi>)"
-  have "wf_pre_total_state ?\<phi>'"
-    apply (rule wf_pre_total_state_1[where ?\<phi>=\<phi>])
-    by simp
-  thus "get_hh_total (Abs_total_state ?\<phi>') = (get_hh_total \<phi>)(l1 := v)"
-    by (simp add: Abs_total_state_inverse_2)
-qed
+  by (simp add: update_hh_loc_total_def)
 
 lemma update_hh_loc_total_lookup_1: "get_hh_total (update_hh_loc_total \<phi> l v) l = v"
   using update_hh_loc_total_fupd
@@ -163,43 +151,32 @@ lemma update_hh_loc_total_lookup_2: "l1 \<noteq> l2 \<Longrightarrow> get_hh_tot
   by (metis fun_upd_apply)
 
 lemma update_hh_loc_total_overwrite: "update_hh_loc_total (update_hh_loc_total \<phi> l v1) l v2 = update_hh_loc_total \<phi> l v2"
-proof -  
-  let ?\<phi>' = "update_hh_loc_total \<phi> l v1"
-  let ?\<phi>'' = "update_hh_loc_total ?\<phi>' l v2"
-  let ?\<phi>_rhs = "update_hh_loc_total \<phi> l v2"
-  have "get_hh_total ?\<phi>'' = (get_hh_total \<phi>)(l := v2)"
-    by (metis fun_upd_upd update_hh_loc_total_fupd)
-  hence A:"get_hh_total ?\<phi>'' = get_hh_total (update_hh_loc_total \<phi> l v2)"
-    by (metis update_hh_loc_total_fupd)
-  show ?thesis
-    apply (rule total_state_eq)
-     apply (simp only: update_hh_loc_total_m_eq)
-    apply (rule total_heap_eq)
-     apply (rule A)
-    apply (simp only: update_hh_loc_total_hp_eq)
-    done
-qed
+  by (simp add: update_hh_loc_total_def)
+
+fun get_h_total_full :: "'a full_total_state \<Rightarrow> 'a total_heap \<times> 'a predicate_heap"
+  where "get_h_total_full \<omega> = (get_hh_total_full \<omega>, get_hp_total_full \<omega>)"
 
 fun update_hh_loc_total_full :: "'a full_total_state \<Rightarrow> heap_loc \<Rightarrow> 'a val \<Rightarrow> 'a full_total_state"
-  where "update_hh_loc_total_full \<omega> l v = (get_store_total \<omega>, get_trace_total \<omega>, update_hh_loc_total (get_total_full \<omega>) l v )"
+  where "update_hh_loc_total_full \<omega> l v = 
+        \<omega>\<lparr> get_total_full := update_hh_loc_total (get_total_full \<omega>) l v \<rparr>"
 
 lemma update_hh_loc_total_full_lookup_1: "get_hh_total_full (update_hh_loc_total_full \<phi> l v) l = v"
-  by (metis get_hh_total_full.simps get_total_full.simps snd_conv update_hh_loc_total_full.simps update_hh_loc_total_lookup_1)
+  by (simp add: update_hh_loc_total_fupd)
 
 lemma update_hh_loc_total_full_lookup_2: "l1 \<noteq> l2 \<Longrightarrow> get_hh_total_full (update_hh_loc_total_full \<phi> l1 v) l2 = get_hh_total_full \<phi> l2"
-  by (metis get_hh_total_full.simps get_total_full.simps snd_conv update_hh_loc_total_full.simps update_hh_loc_total_lookup_2)
+  by (simp add: update_hh_loc_total_lookup_2)
 
 lemma update_hh_loc_total_overwrite_full: "update_hh_loc_total_full (update_hh_loc_total_full \<omega> l v1) l v2 = update_hh_loc_total_full \<omega> l v2"
-  oops
+  by (simp add: update_hh_loc_total_overwrite)
   
 fun update_mh_total_full :: "'a full_total_state \<Rightarrow> mask \<Rightarrow> 'a full_total_state"
-  where "update_mh_total_full \<omega> mh = (get_store_total \<omega>, get_trace_total \<omega>, update_mh_total (get_total_full \<omega>) mh)"
+  where "update_mh_total_full \<omega> mh = \<omega>\<lparr> get_total_full :=  update_mh_total (get_total_full \<omega>) mh \<rparr>"
 
 fun update_mp_total_full :: "'a full_total_state \<Rightarrow> 'a predicate_mask \<Rightarrow> 'a full_total_state"
-  where "update_mp_total_full \<omega> mp = (get_store_total \<omega>, get_trace_total \<omega>, update_mp_total (get_total_full \<omega>) mp)"
+  where "update_mp_total_full \<omega> mp = \<omega>\<lparr> get_total_full := update_mp_total (get_total_full \<omega>) mp \<rparr>"
 
 lemma update_hh_loc_total_full_mask_same: "get_mh_total_full (update_hh_loc_total_full \<omega> l v) = get_mh_total_full \<omega>"
-  by (metis get_total_full.simps get_mh_total_full.simps snd_conv update_hh_loc_total_full.simps update_hh_loc_total_mh_eq)
+  by (simp add: update_hh_loc_total_mh_eq)
 
 lemma get_update_mh_total_full: 
   assumes "wf_mask_simple m0"
@@ -209,8 +186,9 @@ lemma get_update_mh_total_full:
 
 lemma update_mh_total_full_same:
   "(update_mh_total_full \<omega> (get_mh_total_full \<omega>)) = \<omega>"
-  by (simp add: update_mh_total_def Rep_total_state_inverse)
+  by (simp add: update_mh_total_def)
 
+(*
 lemma update_mp_total_h_eq: 
   shows "get_h_total (update_mp_total \<phi> m) = get_h_total \<phi>"
   by (metis Abs_total_state_inverse_2 fst_conv get_h_pre_total.simps get_h_total.elims get_m_pre_total.simps get_mask_total_wf snd_conv update_mp_total_def wf_pre_total_state.simps)
@@ -232,16 +210,30 @@ lemma update_mh_total_full_hh_eq:
   shows "get_h_total_full (update_mh_total_full \<phi> m) = get_h_total_full \<phi>"
   using assms update_mh_total_h_eq
   by auto
+*)
 
 lemma update_mh_total_full_multiple: 
-  assumes "wf_mask_simple m0"
   shows   "update_mh_total_full (update_mh_total_full \<omega> m0) m1 = update_mh_total_full \<omega> m1"
-  using assms
-  using update_mh_total_multiple by fastforce
+  using update_mh_total_multiple 
+  by (metis full_total_state.select_convs(3) full_total_state.surjective full_total_state.update_convs(3) update_mh_total_full.simps)
+
+
+fun get_m_total_full :: "'a full_total_state \<Rightarrow> mask \<times> 'a predicate_mask"
+  where "get_m_total_full \<omega> = (get_mh_total_full \<omega>, get_mp_total_full \<omega>)"
 
 fun update_m_total_full :: "'a full_total_state \<Rightarrow> mask \<Rightarrow> 'a predicate_mask \<Rightarrow> 'a full_total_state"
   where "update_m_total_full \<omega> m pm = 
-                (get_store_total \<omega>, get_trace_total \<omega>, 
-                 update_mp_total (update_mh_total (get_total_full \<omega>) m) pm)"
+              \<omega>\<lparr> get_total_full := update_mp_total (update_mh_total (get_total_full \<omega>) m) pm \<rparr>"
+
+section \<open>Shifting stores\<close>
+
+fun shift_and_add_state_total :: "'a full_total_state \<Rightarrow> 'a val \<Rightarrow> 'a full_total_state"
+  where 
+    "shift_and_add_state_total \<omega> v = update_store_total \<omega> (shift_and_add (get_store_total \<omega>) v)"
+
+fun unshift_state_total :: "nat \<Rightarrow> 'a full_total_state \<Rightarrow> 'a full_total_state"
+  where
+   "unshift_state_total n \<omega> = update_store_total \<omega> (unshift n (get_store_total \<omega>))"         
+                                                            
 
 end
