TotalViperState.thy
@@ -1,20 +1,8 @@
-section \<open>Viper State with a Total Heap\<close>
+section \<open>A state model for the Viper total heap semantics\<close>
 
 theory TotalViperState
 imports Viper.ValueAndBasicState
 begin
-
-type_synonym 'a total_heap = "heap_loc \<Rightarrow> 'a val"
-type_synonym 'a predicate_mask = "'a predicate_loc \<Rightarrow> prat"
-
-text \<open>For each predicate instance, the state tracks the heap snapshot represented as a subset of
-heap locations and predicate locations. The values of the heap locations are given by the 
-corresponding total heap\<close>
-
-type_synonym 'a predicate_heap = "'a predicate_loc \<Rightarrow> heap_loc set \<times> 'a predicate_loc set"
-
-type_synonym 'a pre_total_state = 
-  "('a total_heap \<times> 'a predicate_heap) \<times> (mask \<times> 'a predicate_mask)"
 
 text \<open> We use the following naming scheme:
 
@@ -30,160 +18,86 @@ lh: heap location
 lp: predicate location
 \<close>
 
+
+type_synonym 'a total_heap = "heap_loc \<Rightarrow> 'a val"
+type_synonym 'a predicate_mask = "'a predicate_loc \<Rightarrow> prat"
+
+text \<open>For each predicate instance, the state tracks the heap snapshot represented as a subset of
+heap locations and predicate locations. The values of the heap locations are given by the 
+corresponding total heap\<close>
+
+type_synonym 'a predicate_heap = "'a predicate_loc \<Rightarrow> heap_loc set \<times> 'a predicate_loc set"
+
 fun get_lhset_pheap :: "'a predicate_heap \<Rightarrow> 'a predicate_loc \<Rightarrow> heap_loc set"
   where "get_lhset_pheap hp lp = fst (hp lp)"
 
 fun get_lpset_pheap :: "'a predicate_heap \<Rightarrow> 'a predicate_loc \<Rightarrow> 'a predicate_loc set"
   where "get_lpset_pheap hp lp = snd (hp lp)"
 
-fun get_h_pre_total :: "'a pre_total_state \<Rightarrow> 'a total_heap \<times> 'a predicate_heap"
-  where "get_h_pre_total \<phi> = fst \<phi>"
-
-fun get_hh_pre_total :: "'a pre_total_state \<Rightarrow> 'a total_heap"
-  where "get_hh_pre_total \<phi> = fst (get_h_pre_total \<phi>)"
-
-fun get_hp_pre_total :: "'a pre_total_state \<Rightarrow> 'a predicate_heap"
-  where "get_hp_pre_total \<phi> = snd (get_h_pre_total \<phi>)"
-
-fun get_m_pre_total :: "'a pre_total_state \<Rightarrow> mask \<times> 'a predicate_mask"
-  where "get_m_pre_total \<phi> = snd \<phi>"
-
-fun get_mh_pre_total :: "'a pre_total_state \<Rightarrow> mask"
-  where "get_mh_pre_total \<phi> = fst (get_m_pre_total \<phi>)"
-
-fun get_mp_pre_total :: "'a pre_total_state \<Rightarrow> 'a predicate_mask"
-  where "get_mp_pre_total \<phi> = snd (get_m_pre_total \<phi>)"
-
-fun wf_pre_total_state :: "'a pre_total_state \<Rightarrow> bool" where
-  "wf_pre_total_state \<phi> \<longleftrightarrow> wf_mask_simple (fst (get_m_pre_total \<phi>))"
-
-(* TODO: Does it make sense to use a typedef here given that we can't express the entire state consistency
-here? *)
-typedef 'a total_state = "{ \<phi> :: 'a pre_total_state |\<phi>. wf_pre_total_state \<phi> }"
-  apply (rule_tac x="((\<lambda>hl. VInt 0, \<lambda>p. ({},{})), (zero_mask, zero_mask))" in exI)
-  apply (simp add: wf_zero_mask)
-  done
-
-setup_lifting type_definition_total_state
+record 'a total_state =
+   get_hh_total :: "'a total_heap"
+   get_hp_total :: "'a predicate_heap"
+   get_mh_total :: "mask"
+   get_mp_total :: "'a predicate_mask"
 
 type_synonym 'a total_trace = "label \<rightharpoonup> 'a total_state"
 type_synonym 'a store = "var \<rightharpoonup> 'a val" (* De Bruijn indices *)
-type_synonym 'a full_total_state = "'a store \<times> 'a total_trace \<times> 'a total_state"
+record 'a full_total_state = (*= "'a store \<times> 'a total_trace \<times> 'a total_state"*)
+  get_store_total :: "'a store"
+  get_trace_total :: "'a total_trace"
+  get_total_full :: "'a total_state"
 
-definition empty_full_total_state :: "'a store \<Rightarrow> 'a total_trace \<Rightarrow> ('a total_heap \<times> 'a predicate_heap) \<Rightarrow> 'a full_total_state"
-  where "empty_full_total_state \<sigma> t h = (\<sigma>, t, Abs_total_state (h, (zero_mask, zero_mask)))"
+definition empty_full_total_state :: "'a store \<Rightarrow> 'a total_trace \<Rightarrow> 'a total_heap \<Rightarrow> 'a predicate_heap \<Rightarrow> 'a full_total_state"
+  where "empty_full_total_state \<sigma> t hh hp =
+   \<lparr> get_store_total =\<sigma>, 
+     get_trace_total = t, 
+     get_total_full = \<lparr> get_hh_total = hh, get_hp_total = hp, get_mh_total = zero_mask, get_mp_total = zero_mask \<rparr> 
+   \<rparr>"
 
-section \<open>Destructors for (full) total state\<close>
 
-(*lift_definition get_heap_total :: "'a total_state \<Rightarrow> 'a total_heap" is "snd" done*)
-(*fun get_m_total :: "'a total_stateotal_full  \<Rightarrow> mask \<times> 'a predicate_mask"
-  where "get_m_total \<phi> = get_m_pre_total (Rep_total_state \<phi>)"*)
+section \<open>Destructors \<close>
 
-subsection \<open>Heap destructors total state\<close>
+subsection \<open>total_state\<close>
 
-fun get_h_total :: "'a total_state \<Rightarrow> 'a total_heap \<times> 'a predicate_heap" 
-  where "get_h_total \<phi> = get_h_pre_total (Rep_total_state \<phi>)"
 
-fun get_hh_total :: "'a total_state \<Rightarrow> 'a total_heap" 
-  where "get_hh_total \<phi> = get_hh_pre_total (Rep_total_state \<phi>)"
-
-fun get_hp_total :: "'a total_state \<Rightarrow> 'a predicate_heap" 
-  where "get_hp_total \<phi> = get_hp_pre_total (Rep_total_state \<phi>)"
-
-lemma get_hh_from_h_total: "get_hh_total \<phi> = fst (get_h_total \<phi>)"
-  by simp
-
-lemma get_hp_from_h_total: "get_hp_total \<phi> = snd (get_h_total \<phi>)"
-  by simp
-
-subsection \<open>Mask destructors total state\<close>
-
-fun get_m_total :: "'a total_state \<Rightarrow> mask \<times> 'a predicate_mask" 
-  where "get_m_total \<phi> = get_m_pre_total (Rep_total_state \<phi>)"
-
-fun get_mh_total :: "'a total_state \<Rightarrow> mask" 
-  where "get_mh_total \<phi> = get_mh_pre_total (Rep_total_state \<phi>)"
-
-fun get_mp_total :: "'a total_state \<Rightarrow> 'a predicate_mask" 
-  where "get_mp_total \<phi> = get_mp_pre_total (Rep_total_state \<phi>)"
-
-lemma get_mask_total_wf: "wf_mask_simple (get_mh_total \<phi>)"
-  using Rep_total_state by auto
-
-lemma get_m_mh_mp_total: "get_m_total \<phi> = (get_mh_total \<phi>, get_mp_total \<phi>)"
-  by simp
-
-lemma get_mh_from_m_total: "get_mh_total \<phi> = fst (get_m_total \<phi>)"
-  by simp
-
-lemma get_mp_from_m_total: "get_mp_total \<phi> = snd (get_m_total \<phi>)"
-  by simp
-
-subsection \<open>Top-level constructors full total state\<close>
-
-fun get_store_total :: "'a full_total_state \<Rightarrow> 'a store" 
-  where "get_store_total \<omega> = fst \<omega>"
-
-fun get_trace_total :: "'a full_total_state \<Rightarrow> 'a total_trace" 
-  where "get_trace_total \<omega> = fst (snd \<omega>)"
-
-fun get_total_full :: "'a full_total_state \<Rightarrow> 'a total_state"
-  where "get_total_full \<omega> = snd (snd \<omega>)"
-
-subsection \<open>Heap destructors full total state\<close>
-
-fun get_h_total_full :: "'a full_total_state \<Rightarrow> 'a total_heap \<times> 'a predicate_heap"
-  where "get_h_total_full \<omega> = get_h_total (get_total_full \<omega>)"
-
-fun get_hh_total_full :: "'a full_total_state \<Rightarrow> 'a total_heap" 
+subsection \<open>full total state\<close>
+fun get_hh_total_full :: "'a full_total_state \<Rightarrow> 'a total_heap"
   where "get_hh_total_full \<omega> = get_hh_total (get_total_full \<omega>)"
 
-fun get_hp_total_full :: "'a full_total_state \<Rightarrow> 'a predicate_heap" 
+fun get_hp_total_full :: "'a full_total_state \<Rightarrow> 'a predicate_heap"
   where "get_hp_total_full \<omega> = get_hp_total (get_total_full \<omega>)"
 
-lemma get_hh_from_h_total_full: "get_hh_total_full \<phi> = fst (get_h_total_full \<phi>)"
-  by simp
+fun get_mh_total_full :: "'a full_total_state \<Rightarrow> mask"
+  where "get_mh_total_full \<omega> = get_mh_total (get_total_full \<omega>)"
 
-lemma get_hp_from_h_total_full: "get_hp_total_full \<phi> = snd (get_h_total_full \<phi>)"
-  by simp
+fun get_mp_total_full :: "'a full_total_state \<Rightarrow> 'a predicate_mask"
+  where "get_mp_total_full \<omega> = get_mp_total (get_total_full \<omega>)"
 
-subsection \<open>Mask destructors full total state\<close>
 
-fun get_m_total_full :: "'a full_total_state \<Rightarrow> mask \<times> 'a predicate_mask"
-  where "get_m_total_full \<omega> = get_m_total (get_total_full \<omega>)"
-
-fun get_mh_total_full :: "'a full_total_state \<Rightarrow> mask" where "get_mh_total_full \<omega> = get_mh_total (get_total_full \<omega>)"
-
-fun get_mp_total_full :: "'a full_total_state \<Rightarrow> 'a predicate_mask" where "get_mp_total_full \<omega> = get_mp_total (get_total_full \<omega>)"
-
-lemma get_mh_from_m_total_full: "get_mh_total_full \<phi> = fst (get_m_total_full \<phi>)"
-  by simp
-
-lemma get_mp_from_m_total_full: "get_mp_total_full \<phi> = snd (get_m_total_full \<phi>)"
-  by simp
 
 section \<open>Lemmas for proving equality of states\<close>
 
+(*
 lemma total_mask_eq:
   assumes "get_mh_total \<phi> = get_mh_total \<phi>'" and
           "get_mp_total \<phi> = get_mp_total \<phi>'" 
   shows "get_m_total \<phi> = get_m_total \<phi>'"
   using assms
-  by (metis get_m_total.simps get_mh_pre_total.simps get_mh_total.simps get_mp_pre_total.simps get_mp_total.simps surjective_pairing)
+  by (metis get_m_mh_mp_total)
 
 lemma total_heap_eq:
   assumes "get_hh_total \<phi> = get_hh_total \<phi>'" and
           "get_hp_total \<phi> = get_hp_total \<phi>'" 
   shows "get_h_total \<phi> = get_h_total \<phi>'"
   using assms
-  by (metis get_h_total.elims get_hh_pre_total.simps get_hh_total.elims get_hp_pre_total.simps get_hp_total.elims prod_eqI)
+  by (simp add: prod_eq_iff)
 
 lemma total_state_eq:
   assumes "get_m_total \<phi> = get_m_total \<phi>'" and
           "get_h_total \<phi> = get_h_total \<phi>'"
   shows "\<phi> = \<phi>'"
   using assms
-  by (metis Rep_total_state_inverse get_h_pre_total.simps get_h_total.simps get_m_pre_total.simps get_m_total.simps prod_eqI)
+  by (simp add: prod_eq_iff)
 
 lemma full_total_state_eq: 
   assumes "get_store_total \<omega> = get_store_total \<omega>'" and
@@ -201,10 +115,11 @@ lemma full_total_state_eq_2:
         shows "\<omega> = \<omega>'"
   using assms full_total_state_eq
   by (metis get_h_total_full.elims get_m_total_full.elims total_state_eq)
-
+*)
+(*
 lemma get_mask_total_full_wf: "wf_mask_simple (get_mh_total_full \<omega>)"
   using get_mask_total_wf
   by simp
-
+*)
 
 end
